\documentclass{article}
\usepackage{scibook}
\usepackage{scigeneral}

\title{Notes on the project ParametricAcousticArray}

\usepackage{tabularx}

\begin{document}

\maketitle

\tableofcontents

\section{List of Symbols}

\begin{tabular}{p{4cm}p{10cm}}
	Symbols & Descriptions \\
	$a$ & radius of the source \\
	$c_0$ & isentropic speed of sound at ambient values of pressure and density\\
	$f_1,f_2$ & $f_1= N_1f\st{b},f_2=N_2f\sb{b}$,  primary frequencies\\
	$f\st{b}$ & $=\gcd{f_2-f_1}$, basic frequency\\
	$f\st{m}$ & $=(f_1+f_2)/2$, mean primary frequency\\
	$k$ & $ = 2\uppi f/c_0$  wavenumber\\
	$k\st{m}$ & $=(k_1+k_2)/2$  wavenumber of the mean primary frequency\\
	$l\st{D}$ & $=(\beta k \oldeps)^{-1}$, shock formation distance of a plane wave\\
	$L_x, L_y$ & the size of the rectangular transducer in $x,y$ direction, and $L_y\geq L_x$\\
	$N\st{m}$ & $= (N_1+N_2)/2$\\
	$p$ & pressure\\
	$p_0$ & ambient pressure\\
	$\bar{p}$ & $=(p-p_0)/P_0$, acoustic pressure normalized to $P_0$\\
	$P_0$ & $\rho_0 c_0 v_0$, acoustic pressure peak amplitude on the source\\
	$R\st{D}$ &$=ka^2/2 = \uppi a^2/\lambda$, Rayleigh distance of primary frequency\\
	$R\st{Dm}$ &$=k\st{m}a^2/2 = \uppi a^2/\lambda\st{m}$, Rayleigh distance of mean primary frequency\\
	$t$ & time\\
	$\vb{u}$ & $=(u_x,u_y) = \vb{r}/L_y=(x,y)/L_y$\\
	$v_0$ & characteristic velocity peak amplitude on the source\\
	$x,y,z$ & dimensional coordinates, $z$ along the direction of propagation\\
	$\vb{r}$ & $(x,y)$\\
	$r$ & $|\vb{r}|$\\
	$\alpha$ &absorption coefficient, in Neper per meter\\
	$\beta$ & parameter of nonlinearity\\
	$\oldeps$ & $=u_0/c_0$, Mach number\\
	$\sigma$ & $=z/R\st{D}$, nondimensional $z$ \\
	$\sigma\st{D}$ & $=l\st{D}/R\st{D}$\\
	$\sigma\st{Dm}$ & $=l\st{Dm}/R\st{Dm}$\\
	$\chi$ & $=x/R\st{Dm}$\\
	$\psi$ & $=y/R\st{Dm}$\\
	$\gamma$ & $=L_y/L_x$, the aspect ratio\\
	$\laplacian_{x,y}$ & $\displaystyle=\pdv[2]{x} + \pdv[2]{y}$\\
	$\laplacian_{u}$ & $\displaystyle \pdv[2]{\vb{u}} = \frac{1}{u} \pdv{u} \qty(u \pdv{u})$\\
	% $\laplacian_{\vb{u}}$ & $\displaystyle \pdv[2]{\bm{\xi}} = \frac{1}{\xi} \pdv{\xi} \qty(\xi \pdv{\xi})$\\
	$\laplacian_{\chi,\psi}$ & $\displaystyle=\pdv[2]{\chi} + \pdv[2]{\psi}$\\
\end{tabular}

\section{Theoretical Model and Analytical Solutions}
\subsection{KZK Equation}
Nonlinear propagation of finite amplitude sound waves in dissipative and homogenous fluid is decribed by the following KZK equation: 
\begin{align}
	\pdv{\bar{p} }{\sigma}{\tau}= \alpha R\st{D} \pdv[3]{\bar{p} }{\tau} +\frac14 \laplacian_\perp \bar{p} + \frac{1}{2\sigma\st{D}} \pdv[2]{ (\bar{p})^2}{\tau}
	\label{eq:kzk}
\end{align}

If the source is bifrequency, i.e.
\begin{align}
	f_i = N_i f\st{b}\qc N_i \in \N^+\qc i = 1,2
\end{align}

\subsubsection{Rectangular profile}
The Eq. (\ref{eq:kzk}) is written as

\begin{align}
	\pdv{\bar{p} }{\sigma}{\tau}= \alpha R\st{D} \pdv[3]{\bar{p} }{\tau} +
	\frac{1}{\uppi \gamma} \laplacian_u \bar{p} + \frac{1}{2\sigma\st{D}} \pdv[2]{ (\bar{p})^2}{\tau}
	\label{eq:kzk_rect}
\end{align}

The transformations are:

\begin{align}
	\sigma\st{m} = z/R\st{Dm}\qc
	T = (1+\sigma\st{m})\bar{p}\qc
	\tau\st{m} = \tau - \frac{\uppi \gamma}{4} \frac{\xi^2}{N\st{m} (1+\sigma\st{m})}\qc
	(\chi, \psi) = \frac{(u_x,u_y)}{1+\sigma\st{m}}
\end{align}

Then, the transformed KZK equation is obtained by Eq. (\ref{eq:kzk_rect}) 
\begin{align}
	\pdv{T}{\sigma\st{m}}{\tau\st{m}} 
	= 
	\frac{\alpha\st{m}}{N\st{m}^2} R\st{Dm} \pdv[3]{T}{\tau\st{m}}
	+ \frac{N\st{m}}{\uppi \gamma(1+\sigma\st{m})^2} \laplacian_{\chi, \psi} T
	+\frac{1}{2N\st{m}\sigma\st{Dm}(1+\sigma\st{m})}
	\pdv[2]{(T^2)}{\tau\st{m}}
	\label{eq:kzk_rect_tbe}
\end{align}

\subsection{Spectral Solutions}

A solution of Eq. (\ref{eq:kzk_rect}) is sought in the form of a Fourier series
\begin{align}
	\label{eq:fourier}
	\bar{p} = \sum_{n=1}^\infty (g_n \sin n\tau + h_n \cos n\tau ) = \sum_{n=1}^\infty \bar{p}_n
\end{align}
where $g_n$ and $h_n$ are functions of spatial coordinates.

The solution of Eq. (\ref{eq:kzk_rect_tbe}) is 
\begin{align}
	T = \sum_{n=1}^\infty [g_n(\chi,\psi,\sigma\st{m}) \sin n\tau\st{m} 
		+ h_n(\chi,\psi,\sigma\st{m}) \cos n\tau\st{m} ] 
	= \sum_{n=1}^\infty T_n
\end{align}

\subsection{Coupled PDEs}
We thus obtain the following set of coupled partial differential equations for $g_n$ and $h_n$.

\subsubsection{Rectangular Profile}
\begin{align}
	\pdv{g_n}{\sigma} = - \alpha_n R\st{Dm} g_n &+
	\frac{1}{\uppi \gamma n(1+\sigma\st{m})^2} \laplacian_{\chi,\psi} h_n 
	+ \frac{n}{2N\st{m}\sigma\st{Dm}(1+\sigma\st{m})}\nonumber \\
	&\times \qty[\frac12 \sum_{m=1}^{n-1} (g_m g_{n-m} - h_m h_{n-m}) - \sum_{m=n+1}^\infty (g_{m-n}g_m+h_{m-n}h_m) ]\label{eq:gn_pdv_rect}\\
	\pdv{h_n}{\sigma} = - \alpha_n R\st{Dm} h_n &- \frac{1}{\uppi \gamma n(1+\sigma\st{m})^2} \laplacian_{\chi,\psi} g_n
	+ \frac{n}{2N\st{m}\sigma\st{Dm}(1+\sigma\st{m})} \nonumber \\
	&\times \qty[\sum_{m=1}^{n-1} g_m h_{n-m} + \sum_{m=n+1}^\infty (h_{m-n}g_m-g_{m-n}h_m) ]\label{eq:hn_pdv_rect}
\end{align}

\subsection{Boundary Conditions}
The boundary condition for $g_n$ and $h_n$ at $\sigma = \sigma\st{m}=0$ is 
$$
g_n = \frac1\uppi \int_{-\uppi}^\uppi c \sin n\tau\st{m} \dd{\tau\st{m}}$$
$$
h_n = \frac1\uppi \int_{-\uppi}^\uppi c \cos n\tau\st{m} \dd{\tau\st{m}}$$

\subsubsection{Circular Profile}
The boundary condition at $\sigma=\sigma\st{m}=0$ is 
\begin{align}
	\bar{p} (\sigma\st{m}=0, \bm{\xi},\tau) = c(\bm{\xi}, \tau)
\end{align}

Suppose it is 
\begin{align}
	\bar{p} (\sigma\st{m} =0,\bm{\xi}, \tau) = c_1(\bm{\xi}) \sin N_1 \tau
	+c_2(\bm{\xi}) \sin N_2\tau
\end{align}

\subsubsection{Rectangular Profile}
The boundary condition at $\sigma=\sigma\st{m}=0$ is 
\begin{align}
	\bar{p} (\sigma\st{m}=0, \vb{u},\tau) = c(\vb{u}, \tau)
\end{align}

Suppose it is 
\begin{align}
	\bar{p} (\vb{u},\sigma\st{m} =0, \tau) &= c_1(\vb{u}) \sin N_1 \tau
	+c_2(\vb{u}) \sin N_2\tau \\
	& = c_1(\vb{u}) \qty[\cos\qty(\frac{\uppi \gamma N_1}{4N\st{m}} \xi^2)\sin N_1 \tau\st{m}
	+ \sin \qty(\frac{\uppi \gamma N_1}{4N\st{m}}\xi^2)\cos N_1 \tau\st{m}] \nonumber \\
	&+ c_2(\vb{u}) \qty[\cos\qty(\frac{\uppi \gamma N_1}{4N\st{m}} \xi^2)\sin N_2\tau\st{m}
	+ \sin \qty(\frac{\uppi \gamma N_1}{4 N\st{m}}\xi^2)\cos N_2\tau\st{m}]
\end{align}

Then
\begin{align}
	g_{N_i} (\chi, \psi, \sigma\st{m}=0) = c_i(\chi,\psi) \cos 
	\qty[\frac{\uppi \gamma N_i}{4 N\st{m}} (\chi^2 +\psi^2)]\qc i = 1,2\\
	h_{N_i} (\chi, \psi, \sigma\st{m}=0) = c_i(\chi,\psi) \sin 
	\qty[\frac{\uppi \gamma N_i}{4 N\st{m}} (\chi^2 +\psi^2)]\qc i=1,2\\
	g_n(\chi,\psi, \sigma\st{m}=0) = h_n(\chi,\psi,\sigma\st{m}=0) = 0\qc 
	n \neq N_1, N_2
\end{align}

\section{Numerical Methods}

\subsection{Discretization}
\subsubsection{Rectangular Profile}
$$
\sigma_i = i\Delta \sigma\qc i=0,1, \cdots, I-1, I\qc \sigma_0 = 0\qc \sigma_I = \sigma_\text{max}\qc \Delta\sigma = \frac{\sigma\st{max}}{I}
$$
$$
\chi_j = j\Delta \chi\qc j=0,1, \cdots, J-1, J\qc \chi_0 = 0\qc \chi_J = 
\chi_\text{max}\qc \Delta\chi = \frac{\chi\st{max}}{J}
$$
$$
\psi_k = k\Delta \psi\qc k=0,1, \cdots, K-1, K\qc \psi_0 = 0\qc \psi_K = \psi_\text{max}\qc \Delta\psi = \frac{\psi\st{max}}{K}
$$


For $\pdv*{g_n}{\sigma}$ or $\pdv*{h_n}{\sigma}$, we adopt Backward Implicit
Finite Difference

\begin{align}
	\left. \pdv{g_n(\chi,\psi,\sigma\st{m})}{\sigma\st{m}}\right|_{i,j,k} 
	= \frac{g_n^{i,j,k} - g_n^{i-1,j,k}}{\Delta \sigma\st{m}}\qc
	i = 1,2, \cdots, I
\end{align}

where
\begin{align}
	g_n^{i,j,k} \approx g_n(\chi_j,\psi_k,\sigma_{\mathrm{m},i}) \nonumber \\
	h_n^{i,j,k} \approx h_n(\chi_j,\psi_k,\sigma_{\mathrm{m},i}) 
\end{align}

For $\laplacian_{\chi,\psi} g_n$ or $\laplacian_{\chi,\psi} h_n$, 4 cases
are considered:

(1) $j = 1,2,\cdots,J-1,$ and $k = 1,2,\cdots,K-1$
\begin{align}
	\left. \laplacian_{\chi,\psi}\right|_{i,j,k}
	= \frac{g_n^{i,j-1,k} - 2g_n^{i,j,k} + g_n^{i,j+1,k}}{(\Delta \chi)^2}
	+ \frac{g_n^{i,j,k-1} - 2g_n^{i,j,k} + g_n^{i,j,k+1}}{(\Delta \psi)^2}
\end{align}

(2) $j = 1,2,\cdots,J-1,$ and $k = 0$
\begin{align}
	\left. \laplacian_{\chi,\psi}\right|_{i,j,0}
	= \frac{g_n^{i,j-1,0} - 2g_n^{i,j,0} + g_n^{i,j+1,0}}{(\Delta \chi)^2}
	+ \frac{-2g_n^{i,j,0} + 2g_n^{i,j,1}}{(\Delta \psi)^2}
\end{align}

(3) $j = 0,$ and $k = 1,2,\cdots,K-1$
\begin{align}
	\left. \laplacian_{\chi,\psi}\right|_{i,0,k}
	= \frac{-2g_n^{i,0,k} + 2g_n^{i,1,k}}{(\Delta \chi)^2}
	+ \frac{g_n^{i,0,k-1} - 2g_n^{i,0,k} + g_n^{i,0,k+1}}{(\Delta \psi)^2}
\end{align}

(4) $j = 0,$ and $k =0$

\begin{align}
	\left. \laplacian_{\chi,\psi}\right|_{i,0,0}
	= \frac{-2g_n^{i,0,0} + 2g_n^{i,1,0}}{(\Delta \chi)^2}
	+ \frac{-2g_n^{i,0,0} + 2g_n^{i,0,1}}{(\Delta \psi)^2}
\end{align}

where the symmetric conditions are used
\begin{align}
	\left.\pdv{g_n}{\chi}\right|_{\chi=0} = \left.\pdv{h_n}{\chi}\right|_{\chi=0} = 0\qc n= 1,2,\cdots,N\nonumber\\
	\left. \pdv{g_n}{\psi}\right|_{\psi=0} = \left. \pdv{h_n}{\psi}\right|_{\psi=0} = 0\qc n= 1,2,\cdots,N
\end{align}


Discrete Eq. (\ref{eq:gn_pdv_rect}) and Eq. (\ref{eq:hn_pdv_rect}), we have

(1) $j = 1,2,\cdots,J-1,$ and $k = 1,2,\cdots,K-1$
\begin{align}
	g_n^{i,j,k}-g_n^{i-1,j,k} = - \Delta\sigma\st{m}&\alpha_n R\st{Dm} g_n^{i,j,k}
	+\mathcal{G}_n^{i-1,j,k}
	+\frac{\Delta\sigma_{\mathrm{m}}}{\uppi \gamma n(1+\sigma_{\mathrm{m},i})^2} \nonumber\\
	&\times\qty[\frac{h_n^{i,j-1,k}-2h_n^{i,j,k}+h_n^{i,j+1,k}}{(\Delta \chi)^2}
	+ \frac{h_n^{i,j,k-1} - 2h_n^{i,j,k} +h_n^{i,j,k+1}}{(\Delta \psi)^2}]\\
	h_n^{i,j,k}-h_n^{i-1,j,k} = - \Delta\sigma\st{m}&\alpha_n R\st{Dm} h_n^{i,j,k}
	+\mathcal{H}_n^{i-1,j,k}
	-\frac{\Delta\sigma\st{m}}{\uppi \gamma n(1+\sigma_{\mathrm{m},i})^2} \nonumber\\
	&\times\qty[\frac{g_n^{i,j-1,k}-2g_n^{i,j,k}+g_n^{i,j+1,k}}{(\Delta \chi)^2}
	+ \frac{g_n^{i,j,k-1} - 2g_n^{i,j,k} +g_n^{i,j,k+1}}{(\Delta \psi)^2}]
\end{align}

(2) $j = 1,2,\cdots,J-1,$ and $k = 0$

\begin{align}
	g_n^{i,j,0}-g_n^{i-1,j,0} = - \Delta\sigma\st{m}&\alpha_n R\st{Dm} g_n^{i,j,0}
	+\mathcal{G}_n^{i-1,j,0}
	+\frac{\Delta\sigma_{\mathrm{m}}}{\uppi \gamma n(1+\sigma_{\mathrm{m},i})^2} \nonumber\\
	&\times\qty[\frac{h_n^{i,j-1,0}-2h_n^{i,j,0}+h_n^{i,j+1,0}}{(\Delta \chi)^2}
	+ \frac{-2h_n^{i,j,0} + 2h_n^{i,j,1} }{(\Delta \psi)^2}]\\
	h_n^{i,j,0}-h_n^{i-1,j,0} = - \Delta\sigma\st{m}&\alpha_n R\st{Dm} h_n^{i,j,0}
	+\mathcal{H}_n^{i-1,j,0}
	-\frac{\Delta\sigma_{\mathrm{m}}}{\uppi \gamma n(1+\sigma_{\mathrm{m},i})^2} \nonumber\\
	&\times\qty[\frac{g_n^{i,j-1,0}-2g_n^{i,j,0}+g_n^{i,j+1,0}}{(\Delta \chi)^2}
	+ \frac{-2g_n^{i,j,0} + 2g_n^{i,j,1} }{(\Delta \psi)^2}]
\end{align}

(3) $j = 0,$ and $k = 1,2,\cdots,K-1$
\begin{align}
	g_n^{i,0,k}-g_n^{i-1,0,k} = - \Delta\sigma\st{m}&\alpha_n R\st{Dm} g_n^{i,0,k}
	+\mathcal{G}_n^{i-1,0,k}
	+\frac{\Delta\sigma_{\mathrm{m}}}{\uppi \gamma n(1+\sigma_{\mathrm{m},i})^2} \nonumber\\
	&\times\qty[\frac{-2h_n^{i,0,k}+2h_n^{i,1,k}}{(\Delta \chi)^2}
	+ \frac{h_n^{i,0,k-1} - 2h_n^{i,0,k} +h_n^{i,0,k+1}}{(\Delta \psi)^2}]\\
	h_n^{i,0,k}-h_n^{i-1,0,k} = - \Delta\sigma\st{m}&\alpha_n R\st{Dm} h_n^{i,0,k}
	+\mathcal{H}_n^{i-1,0,k}
	-\frac{\Delta\sigma\st{m}}{\uppi \gamma n(1+\sigma_{\mathrm{m},i})^2} \nonumber\\
	&\times\qty[\frac{-2g_n^{i,0,k}+2g_n^{i,1,k}}{(\Delta \chi)^2}
	+ \frac{g_n^{i,0,k-1} - 2g_n^{i,0,k} +g_n^{i,0,k+1}}{(\Delta \psi)^2}]
\end{align}

(4) $j = 0,$ and $k =0$
\begin{align}
	g_n^{i,0,0}-g_n^{i-1,0,0} = - \Delta\sigma\st{m}&\alpha_n R\st{Dm} g_n^{i,0,0}
	+\mathcal{G}_n^{i-1,0,0}
	+\frac{\Delta\sigma_{\mathrm{m}}}{\uppi \gamma n(1+\sigma_{\mathrm{m},i})^2} \nonumber\\
	&\times\qty[\frac{-2h_n^{i,0,0}+2h_n^{i,1,0}}{(\Delta \chi)^2}
	+ \frac{-2h_n^{i,0,0} + 2h_n^{i,0,1} }{(\Delta \psi)^2}]\\
	h_n^{i,0,0}-h_n^{i-1,0,0} = - \Delta\sigma\st{m}&\alpha_n R\st{Dm} h_n^{i,0,0}
	+\mathcal{H}_n^{i-1,0,0}
	-\frac{\Delta\sigma\st{m}}{\uppi \gamma n(1+\sigma_{\mathrm{m},i})^2} \nonumber\\
	&\times\qty[\frac{-2g_n^{i,0,0}+2g_n^{i,1,0}}{(\Delta \chi)^2}
	+ \frac{-2g_n^{i,0,0} + 2g_n^{i,0,1} }{(\Delta \psi)^2}]
\end{align}

where 
\begin{align}
	\mathcal{G}_n^{i,j,k} &= \frac{n\Delta \sigma\st{m}}{2N\st{m} \sigma\st{Dm}
	(1+\sigma_{\mathrm{m},i})}
	\qty[\frac12 \sum_{m=1}^{n-1} (g_m^{i,j,k} g_{n-m}^{i,j,k}-
	h_{m}^{i,j,k} h_{n-m}^{i,j,k}) - 
	\sum_{n+1}^N (g_{m}^{i,j,k}g_{m-n}^{i,j,k} + h_{m}^{i,j,k} h_{m-n}^{i,j,k})]\\
	\mathcal{H}_n^{i,j,k} &= \frac{n\Delta \sigma\st{m}}{2N\st{m} \sigma\st{Dm}
	(1+\sigma_{\mathrm{m},i})}
	\qty[\sum_{m=1}^{n-1} g_m^{i,j,k} h_{n-m}^{i,j,k}
	+\sum_{n+1}^N (g_{m}^{i,j,k}h_{m-n}^{i,j,k} - h_{m}^{i,j,k} g_{m-n}^{i,j,k})]
\end{align}
\section{Legacy}


\subsection{Matrix Form}
\begin{align}
	I_{2(J-1)} \mqty[G_n^i-G_n^{i-1}\\ H_n^i-H_n^{i-1}] 
= \mqty[B_{(J-1)\times(J-1)} & A_{(J-1)\times(J-1)}\\ -A_{(J-1)\times(J-1)} & B_{(J-1)\times(J-1)}] \mqty[G_n^i\\ H_n^i] 
+\mqty[\mathcal{H}_n^i\\ \mathcal{G}_n^i]
+\mqty[S_n^{i-1}\\ T_n^{i-1}]
\end{align}
$$
(i=1,2,\cdots, I-1,I)
$$

It can be written as

\begin{align}
	\qty(I_{2(J-1)} - \mqty[B&A\\ -A&B] ) \mqty[G_n^i\\H_n^i] = I_{2(J-1)} \mqty[G_n^{i-1}\\ H_n^{i-1}] 
+\mqty[\mathcal{H}_n^i\\ \mathcal{G}_n^i]
+\mqty[S_n^{i-1}\\ T_n^{i-1}]
\end{align}

where
\begin{align}
	G_n^i = \mqty[g_n^{i,1}\\ g_n^{i,2} \\ \vdots \\ g_n^{i,J-1}]\qc 
	G_n^{i-1} = \mqty[g_n^{i-1,1}\\ g_n^{i-1,2} \\ \vdots \\ g_n^{i-1,J-1}]\qc 
	H_n^i = \mqty[h_n^{i,1}\\ h_n^{i,2} \\ \vdots \\ h_n^{i,J-1}]\qc 
	H_n^{i-1} = \mqty[h_n^{i-1,1}\\ h_n^{i-1,2} \\ \vdots \\ h_n^{i-1,J-1}]
\end{align}

\begin{align}
	\mathcal{G}_n^i = \mqty[a_1 g_n^{i,0}\\ O_{(J-3)\times 1} \\ b_{J-1} g_n^{i,J}]\qc
	\mathcal{H}_n^i = \mqty[a_1 h_n^{i,0}\\ O_{(J-3)\times 1} \\ b_{J-1} h_n^{i,J}]\qc 
	h_n^{i,J} = h_n(\sigma_i, \xi_J) = h_n(\sigma_i,\xi\st{max}) = 0
\end{align}

\begin{align}
	A = \mqty[q & b_1 \\ a_2 & q & b_2 \\ & & & & \vdots \\ & & & & & a_{J-2}& q & b_{J-2}\\ &&&&&&a_{J-1}&q]\qc
	\begin{cases}
		a_j = (1-0.5/j)\dfrac{\Delta \sigma}{4n(\Delta \xi)^2} \\
		b_j = (1+0.5/j)\dfrac{\Delta \sigma}{4n(\Delta \xi)^2} \\
		q = -\dfrac{\Delta \sigma }{2n(\Delta \xi)^2}
	\end{cases} j=1,2,\cdots, J-1
\end{align}

\begin{align}
	B = -\Delta \sigma \alpha_n R\st{D} I_{J-1}
\end{align}

\begin{align}
	S_n^{i-1} = \mqty[S_n^{i-1,1} \\ S_n^{i-1,2} \\ \vdots \\ S_n^{i-1,J-1}]\qc
	T_n^{i-1} = \mqty[T_n^{i-1,1} \\ T_n^{i-1,2} \\ \vdots \\ T_n^{i-1,J-1}]
\end{align}

\begin{align}
	S_n^{i-1,j} = \Delta \sigma n\frac{R\st{D}}{2l\st{D}}\qty[\frac12\sum_{m=1}^{n-1}(g_m^{i-1,j}g_{n-m}^{i-1,j}-h_m^{i-1,j}h_{n-m}^{i-1,j}) - \sum_{m=n+1}^M (g_{m-n}^{i-1,j} g_m^{i-1,j}+h_{m-n}^{i-1,j}h_m^{i-1,j})]\\
	T_n^{i-1,j} = \Delta \sigma n\frac{R\st{D}}{2l\st{D}}\qty[\frac12\sum_{m=1}^{n-1}(h_m^{i-1,j}g_{n-m}^{i-1,j}+g_m^{i-1,j}h_{n-m}^{i-1,j}) + \sum_{m=n+1}^M (h_{m-n}^{i-1,j} g_m^{i-1,j}-g_{m-n}^{i-1,j}h_m^{i-1,j})]
\end{align}

\begin{align}
	g_n^{i,0} = (1-\Delta\sigma  \alpha_n R\st{D})g_n^{i-1,0} + \frac{\Delta \sigma}{n(\Delta\xi)^2} (h_n^{i-1,1}-h_n^{i-1,0})+ S_n^{i-1,0}\\
	h_n^{i,0} = (1-\Delta\sigma  \alpha_n R\st{D})h_n^{i-1,0} - \frac{\Delta \sigma}{n(\Delta\xi)^2} (g_n^{i-1,1}-g_n^{i-1,0}) + T_n^{i-1,0}
\end{align}
$$
	(i=1,2,\cdots,I) \nonumber
	$$

\section{Crank-Nicolson Method}
\begin{equation}
\end{equation}

\subsection{Data Set: Kamakura 1989}
\emph{Fig. 6}
$$
\Delta \sigma = 3\times 10^{-4}\qc \sigma\st{max} = 10\qc \Delta \xi = 0.03\qc \xi\st{max} = 6\qc T = 23.7 \celsius\qc h\st{r} = 65.2\%
$$
$$
M=18\qc f_1 = 25 \text{kHz}\qc f_2 = 30 \text{kHz}\qc P_0(25 \text{kHz}) = 109.5 \text{dB}\qc P_0(30 \text{kHz})=108.5 \text{dB}
$$
$$
a = 0.21\si{m}
$$
\end{document}

